Iterator/Lemmas/Combinator.lean
@@ -1,61 +1,10 @@
 import Iterator.Combinators.FilterMap
-
--- section Equivalence
-
--- variable {α : Type u} {m : Type w → Type w'} {β : Type v}
-
--- inductive IterTStep (β : Type v) where
---   | yield : β → IterTStep β
---   | skip : IterTStep β
---   | done : IterTStep β
-
--- inductive IterT (m : Type w → Type w') (β : Type v) : Type w → Type (max v w w' + 1) where
---   | step : ∀ {α}, Nat → (β → α) → IterT m β (IterTStep α)
---   | lift : ∀ {α}, m α → IterT m β α
---   | bind : ∀ {α γ}, IterT m β α → (α → IterT m β γ) → IterT m β γ
-
--- def IterT.interpret [Iterator α m β] [Monad m] (it : α) (γ : Type w) (x : IterT m β γ) : m γ :=
---   go [it] x |>.mapH (fun p => p.1) |>.run
--- where
---   go {δ : Type w} (its : List α) : IterT m β δ → CodensityT m (δ × List α)
---     | .step n f => match its[n]? with
---       | none => pure (.done, its)
---       | some it =>
---         let v := Iterator.step it
---         v.mapH (match · with
---           | .yield it' out _ => (.yield (f out), it' :: its)
---           | .skip it' _ => (.skip, it' :: its)
---           | .done _ => (.done, its))
---     | .lift x => (CodensityT.eval x).mapH (Prod.mk · its)
---     | .bind x f => (go its x) >>= (fun y => go y.2 (f y.1))
-
--- end Equivalence
+import Iterator.Consumers
 
 variable {α : Type u} {m : Type w → Type w'} {β : Type v}
   [Iterator α m β] {_ : ComputableSmall.{w} α} (it : Iter (α := α) m β)
   [Monad m]
   (f : β → CodensityT m (Option β'))
-
--- theorem filterMapMH_step' (it : α) (f : β → IterationT m (Option β')) :
---     Iterator.step (m := m) (Iterator.filterMapMH f it) =
---       (Iterator.step (m := m) it |>.bindH (match · with
---         | .yield it' out h => (f out).computation.mapH (fun x => ⟨match x.val with
---           | none => .skip ⟨it'⟩
---           | some out => .yield ⟨it'⟩ out, .yield it' out, ⟨x.1, rfl, x.2⟩, h⟩)
---         | .skip it' h => pure ⟨.skip ⟨it'⟩, .skip it', rfl, h⟩
---         | .done h => pure ⟨.done, .done, rfl, h⟩)) := by
---   simp [Iterator.filterMapMH, Iterator.step, SimpleIterator.step, computation_matchStepH,
---     IterationT.step, IterationT.mapH, CodensityT.mapH_mapH, IterationT.computation_pure]
---   refine congrArg (CodensityT.bindH _) ?_
---   ext x
---   split
---   · simp
---     refine congrArg (CodensityT.mapH · _) ?_
---     ext y
---     cases y
---     dsimp only
---     split <;> rfl
---   · simp
 
 theorem FilterMapMH.plausible_of_yield_of_none {it' : Iter (α := α) m β} {out : β}
     (h : it.plausible_step (.yield it' out)) :
@@ -143,34 +92,6 @@ theorem filterMapMH_step :
       IterationT.computation_pure, CodensityT.bindH_pure]
     rfl
 
-#exit
-  simp only [plausible_eq_copy
-    (congrArg Iterator.step (inner_toIter ..)),
-    congrArg Iterator.step, congrArg FilterMapMH.inner, inner_toIter]
-
-  simp [Iter.filterMapH, Iter.stepH, Iterator.step]
-  simp [Iter.filterMapMH, Iter.stepH]
-  simp [IterationT.bindH, IterationT.mapH]
-  simp only [plausible_eq_copy
-    (congrArg (Iterator.step (m := m) (α := α))
-      (congrArg FilterMapMH.inner (inner_toIter ..))),
-    congrArg Iterator.step, congrArg FilterMapMH.inner, inner_toIter]
-  simp [Iterator.filterMapMH]
-  simp [toIter, Iter.inner]
-  simp [computation_matchStep, IterationT.computation_pure]
-  rw [Iterator.step_congr <| ComputableSmall.down_up ..]
-  rw [filterMapMH_step']
-  simp [CodensityT.map_eq_mapH, CodensityT.mapH_mapH]
-  simp [Iter.Step.ofInternal.eq_def, PlausibleIterStep.map_map]
-  rw [Iterator.filterMapMH]
-  simp [Iter.stepH, Iterator.step, SimpleIterator.step, Iter.Step.ofInternal]
-
-  simp [Iter.stepH, Iterator.step, SimpleIterator.step, CodensityT.map_eq_mapH, CodensityT.mapH_mapH, Iter.Step.ofInternal]
-
-  simp [CodensityT]
-  ext
-  simp [Iter.stepH, CodensityT.mapH, CodensityT.bindH, Iterator.step, SimpleIterator.step, IterationT.step, Functor.map]
-  let proof : (it.filterMapMH f).stepH = sorry := by
-    simp [Iter.stepH, Iterator.step, SimpleIterator.step, IterationT.mapH, IterationT.computation_pure,
-      CodensityT.map_bindH, IterationT.step]
-    split
+-- TODO: Perhaps we should also carry the small instance around in Iter
+theorem toList_filterMapMH [Finite α m] [ComputableSmall β] :
+    (it.filterMapMH f).toList = it.foldM
