Iterator/Lemmas/Consumer.lean
@@ -1,0 +1,267 @@
+import Iterator.Producers
+import Iterator.Consumers
+import Iterator.Combinators.FilterMap
+
+section Consumers
+
+@[specialize]
+def Iter.induct {α m β} {_ : Iterator α m β} {_ : ComputableSmall α} [Finite α m]
+  (motive : Iter (α := α) m β → Sort x)
+  (step : (it : Iter (α := α) m β) →
+    (ih_yield : ∀ {it' : Iter (α := α) m β} {out : β}, it.plausible_step (.yield it' out) → motive it') →
+    (ih_skip : ∀ {it' : Iter (α := α) m β}, it.plausible_step (.skip it') → motive it' ) →
+    motive it) (it : Iter (α := α) m β) : motive it :=
+  step _ (fun {it' _} _ => Iter.induct motive step it') (fun {it'} _ => Iter.induct motive step it')
+termination_by it.terminationByFinite
+
+theorem Iter.toArray.go.aux₁ [Monad m] [LawfulMonad m] {_ : Iterator α m β} [Finite α m] {_ : ComputableSmall α}
+    {it : Iter (α := α) m β} {b : β} {bs : Array β} :
+    Iter.toArray.go it (#[b] ++ bs) = (#[b] ++ ·) <$> Iter.toArray.go it bs := by
+  induction it, bs using Iter.toArray.go.induct
+  next it bs ih₁ ih₂ =>
+  rw [go, map_eq_pure_bind, go, bind_assoc]
+  refine congrArg (Iter.step it >>= ·) ?_
+  ext step
+  split <;> simp [*]
+
+theorem Iter.toArray.go.aux₂ [Monad m] [LawfulMonad m] {_ : Iterator α m β} [Finite α m] {_ : ComputableSmall α}
+    {it : Iter (α := α) m β} {acc : Array β} :
+    Iter.toArray.go it acc = (acc ++ ·) <$> it.toArray := by
+  rw [← Array.toArray_toList (xs := acc)]
+  generalize acc.toList = acc
+  induction acc with
+  | nil => simp [toArray]
+  | cons x xs ih =>
+    rw [List.toArray_cons, Iter.toArray.go.aux₁, ih]
+    simp only [Functor.map_map, Array.append_assoc]
+
+theorem Iter.toArray_of_step [Monad m] [LawfulMonad m] {_ : Iterator α m β} [Finite α m] {_ : ComputableSmall α}
+    {it : Iter (α := α) m β} :
+    it.toArray = (do
+      match ← it.step with
+      | .yield it' out _ => return #[out] ++ (← it'.toArray)
+      | .skip it' _ => it'.toArray
+      | .done _ => return #[]) := by
+  rw [Iter.toArray, Iter.toArray.go]
+  refine congrArg (_ >>= ·) ?_
+  ext step
+  split <;> simp [Iter.toArray.go.aux₂]
+
+theorem Iter.toList_toArray [Monad m] {_ : Iterator α m β} [Finite α m] {_ : ComputableSmall α}
+    {it : Iter (α := α) m β} :
+    Array.toList <$> it.toArray = it.toList := by
+  simp [Iter.toList]
+
+theorem Iter.toArray_toList [Monad m] [LawfulMonad m] {_ : Iterator α m β} [Finite α m] {_ : ComputableSmall α}
+    {it : Iter (α := α) m β} :
+    List.toArray <$> it.toList = it.toArray := by
+  simp [Iter.toList]
+
+theorem Iter.toList_of_step [Monad m] [LawfulMonad m] {_ : Iterator α m β} [Finite α m] {_ : ComputableSmall α}
+    {it : Iter (α := α) m β} :
+    it.toList = (do
+      match ← it.step with
+      | .yield it' out _ => return out :: (← it'.toList)
+      | .skip it' _ => it'.toList
+      | .done _ => return []) := by
+  simp [← Iter.toList_toArray]
+  rw [Iter.toArray_of_step, map_eq_pure_bind, bind_assoc]
+  refine congrArg (_ >>= ·) ?_
+  ext step
+  split <;> simp
+
+theorem Iter.reverseToList.go.aux₁ [Monad m] [LawfulMonad m] {_ : Iterator α m β} [Finite α m] {_ : ComputableSmall α}
+    {it : Iter (α := α) m β} {b : β} {bs : List β} :
+    Iter.reverseToList.go it (bs ++ [b]) = (· ++ [b]) <$> Iter.reverseToList.go it bs:= by
+  induction it, bs using Iter.reverseToList.go.induct
+  next it bs ih₁ ih₂ =>
+  rw [go, go, map_eq_pure_bind, bind_assoc]
+  refine congrArg (Iter.step it >>= ·) ?_
+  ext step
+  simp only [List.cons_append] at ih₁
+  split <;> simp [*]
+
+theorem Iter.reverseToList.go.aux₂ [Monad m] [LawfulMonad m] {_ : Iterator α m β} [Finite α m] {_ : ComputableSmall α}
+    {it : Iter (α := α) m β} {acc : List β} :
+    Iter.reverseToList.go it acc = (· ++ acc) <$> it.reverseToList := by
+  rw [← List.reverse_reverse (as := acc)]
+  generalize acc.reverse = acc
+  induction acc with
+  | nil => simp [reverseToList]
+  | cons x xs ih => simp [Iter.reverseToList.go.aux₁, ih]
+
+theorem Iter.reverseToList_of_step [Monad m] [LawfulMonad m] {_ : Iterator α m β} [Finite α m] {_ : ComputableSmall α}
+    {it : Iter (α := α) m β} :
+    it.reverseToList = (do
+      match ← it.step with
+      | .yield it' out _ => return (← it'.reverseToList) ++ [out]
+      | .skip it' _ => it'.reverseToList
+      | .done _ => return []) := by
+  simp [Iter.reverseToList]
+  rw [reverseToList.go]
+  refine congrArg (it.step >>= ·) ?_
+  ext step
+  obtain ⟨step, h⟩ := step
+  cases step <;> simp [Iter.reverseToList.go.aux₂]
+
+theorem Iter.reverse_reverseToList [Monad m] [LawfulMonad m] {_ : Iterator α m β} [Finite α m]
+    {_ : ComputableSmall α} {it : Iter (α := α) m β} :
+    List.reverse <$> it.reverseToList = it.toList := by
+  apply Eq.symm
+  induction it using Iter.induct
+  rename_i it ihy ihs
+  rw [reverseToList_of_step, toList_of_step, map_eq_pure_bind, bind_assoc]
+  refine congrArg (_ >>= ·) ?_
+  ext step
+  split <;> simp (discharger := assumption) [ihy, ihs]
+
+end Consumers
+
+section ListIterator
+
+variable {m : Type v → Type v} [Monad m] {β : Type v}
+
+-- theorem List.step_iter_nil :
+--     (([] : List β).iter m).step = pure ⟨.done, .done, sorry, [], sorry⟩
+
+-- private theorem List.toArray_iter.aux {l : List β} {acc : Array β} :
+--     Iter.toArray.go (l.iter m) acc = pure (acc ++ l.toArray) := by
+--   simp [List.iter]
+--   induction l generalizing acc with
+--   | nil =>
+--     rw [Iter.toArray.go]
+--     simp [Iter.step, Iter.stepH, CodensityT.run, CodensityT.mapH, Iterator.step,
+--       IterationT.map_eq_mapH, IterationT.mapH, IterationT.computation_pure, Pure.pure]
+--     simp [Iter.Step.ofInternal, IterationT.Plausible.map, IterStep.map]
+--   | cons x xs ih =>
+--     rw [Iter.toArray.go]
+--     simp [Iter.step, Iter.stepH, CodensityT.run, CodensityT.mapH, Iterator.step,
+--       IterationT.map_eq_mapH, IterationT.mapH, IterationT.computation_pure, Pure.pure,
+--       Iter.Step.ofInternal, IterationT.Plausible.map, IterStep.map, ih]
+
+-- private theorem List.toArray_iter {l : List β} :
+--     Iter.toArray (l.iter m)
+
+end ListIterator
+
+-- section Equivalence
+
+-- variable {α : Type u} {m : Type w → Type w'} {β : Type v}
+
+-- inductive IterTStep (β : Type v) where
+--   | yield : β → IterTStep β
+--   | skip : IterTStep β
+--   | done : IterTStep β
+
+-- inductive IterT (m : Type w → Type w') (β : Type v) : Type w → Type (max v w w' + 1) where
+--   | step : ∀ {α}, Nat → (β → α) → IterT m β (IterTStep α)
+--   | lift : ∀ {α}, m α → IterT m β α
+--   | bind : ∀ {α γ}, IterT m β α → (α → IterT m β γ) → IterT m β γ
+
+-- def IterT.interpret [Iterator α m β] [Monad m] (it : α) (γ : Type w) (x : IterT m β γ) : m γ :=
+--   go [it] x |>.mapH (fun p => p.1) |>.run
+-- where
+--   go {δ : Type w} (its : List α) : IterT m β δ → CodensityT m (δ × List α)
+--     | .step n f => match its[n]? with
+--       | none => pure (.done, its)
+--       | some it =>
+--         let v := Iterator.step it
+--         v.mapH (match · with
+--           | .yield it' out _ => (.yield (f out), it' :: its)
+--           | .skip it' _ => (.skip, it' :: its)
+--           | .done _ => (.done, its))
+--     | .lift x => (CodensityT.eval x).mapH (Prod.mk · its)
+--     | .bind x f => (go its x) >>= (fun y => go y.2 (f y.1))
+
+-- end Equivalence
+
+-- variable {α : Type u} {m : Type w → Type w'} {β : Type v}
+--   [Iterator α m β] {_ : ComputableSmall.{w} α} (it : Iter (α := α) m β)
+--   [Monad m]
+--   (f : β → CodensityT m (Option β'))
+
+-- theorem FilterMapMH.plausible_of_yield_of_none {it' : Iter (α := α) m β} {out : β}
+--     (h : it.plausible_step (.yield it' out)) :
+--     (it.filterMapMH f).plausible_step (.skip (it'.filterMapMH f)) := by
+--   let step : it.Step := .yield it' out h
+--   let internalStep := step.toInternal
+--   simp only [Iter.plausible_step]
+--   refine ⟨.skip (it'.filterMapMH f).inner, by simp [IterStep.map, Iter.filterMapMH], ?_⟩
+--   refine ⟨.yield (it'.filterMapMH f).inner.inner out, ?_, ?_⟩
+--   · exact ⟨none, rfl, True.intro⟩
+--   · simp only [Iter.filterMapMH, Iterator.filterMapMH, inner_toIter]
+--     exact internalStep.property
+
+-- theorem FilterMapMH.plausible_of_yield_of_some {it' : Iter (α := α) m β} {out : β} {out' : β'}
+--     (h : it.plausible_step (.yield it' out)) :
+--     (it.filterMapMH f).plausible_step (.yield (it'.filterMapMH f) out') := by
+--   let step : it.Step := .yield it' out h
+--   let internalStep := step.toInternal
+--   refine ⟨.yield (it'.filterMapMH f).inner out', by simp [IterStep.map, Iter.filterMapMH], ?_⟩
+--   refine ⟨.yield (it'.filterMapMH f).inner.inner out, ?_, ?_⟩
+--   · exact ⟨some out', rfl, True.intro⟩
+--   · simp only [Iter.filterMapMH, Iterator.filterMapMH, inner_toIter]
+--     exact internalStep.property
+
+-- theorem FilterMapMH.plausible_of_skip {it' : Iter (α := α) m β}
+--     (h : it.plausible_step (.skip it')) :
+--     (it.filterMapMH f).plausible_step (.skip (it'.filterMapMH f)) := by
+--   let step : it.Step := .skip it' h
+--   let internalStep := step.toInternal
+--   refine ⟨.skip (it'.filterMapMH f).inner, by simp [IterStep.map, Iter.filterMapMH], ?_⟩
+--   refine ⟨.skip (it'.filterMapMH f).inner.inner, rfl, ?_⟩
+--   simp only [Iter.filterMapMH, Iterator.filterMapMH, inner_toIter]
+--   exact internalStep.property
+
+-- theorem FilterMapMH.plausible_of_done
+--     (h : it.plausible_step .done) :
+--     (it.filterMapMH f).plausible_step .done := by
+--   let step : it.Step := .done h
+--   let internalStep := step.toInternal
+--   refine ⟨.done, by simp [IterStep.map, Iter.filterMapMH], ?_⟩
+--   refine ⟨.done, rfl, ?_⟩
+--   simp only [Iter.filterMapMH, Iterator.filterMapMH, inner_toIter]
+--   exact internalStep.property
+
+-- theorem filterMapMH_step :
+--   (it.filterMapMH f).stepH = (it.stepH.bindH (match · with
+--       | .yield it' out h => (f out).mapH fun
+--           | none => .skip (it'.filterMapMH f) (FilterMapMH.plausible_of_yield_of_none _ _ h)
+--           | some out' => .yield (it'.filterMapMH f) out' (FilterMapMH.plausible_of_yield_of_some _ _ h)
+--       | .skip it' h => pure <| .skip (it'.filterMapMH f) (FilterMapMH.plausible_of_skip _ _ h)
+--       | .done h => pure <| .done (FilterMapMH.plausible_of_done _ _ h))) := by
+--   cases it
+--   simp only [Iter.filterMapMH, Iterator.filterMapMH]
+--   rw [Iter.stepH, CodensityT.mapH_eq_bindH]
+--   rw [Iter.stepH, CodensityT.mapH_eq_bindH]
+--   simp only [plausible_eq_copy
+--     (congrArg Iterator.step (inner_toIter ..)),
+--     congrArg Iterator.step, congrArg FilterMapMH.inner, inner_toIter]
+--   simp only [Iterator.step]
+--   rw [CodensityT.map_eq_mapH, CodensityT.mapH_eq_bindH]
+--   simp only [IterationT.bindH]
+--   simp only [CodensityT.bindH_assoc]
+--   refine congrArg (CodensityT.bindH _ ·) ?_
+--   ext x
+--   simp only [CodensityT.bindH_pure, Iter.Step.ofInternal, IterationT.Plausible.map, IterStep.map]
+--   match h : x with
+--   | ⟨.yield .., h⟩ =>
+--     simp only [matchStep]
+--     simp only [IterationT.mapH, CodensityT.mapH_eq_bindH, monadLift, MonadLift.monadLift,
+--       CodensityT.map_eq_mapH, CodensityT.mapH_eq_bindH, CodensityT.bindH_assoc,
+--       CodensityT.bindH_pure]
+--     refine congrArg (CodensityT.bindH _ ·) ?_
+--     ext y
+--     refine congrArg pure ?_
+--     simp only [IterationT.Plausible.copy, Iter.Step.yield, Iter.Step.skip, Iter.filterMapMH,
+--       Iterator.filterMapMH, inner_toIter]
+--     cases y <;> rfl
+--   | ⟨.skip .., h⟩ =>
+--     simp only [matchStep]
+--     simp only [CodensityT.mapH_eq_bindH, IterationT.computation_pure, CodensityT.bindH_pure,
+--       IterationT.Plausible.copy, Iter.Step.skip, Iter.filterMapMH, Iterator.filterMapMH,
+--       inner_toIter]
+--   | ⟨.done, h⟩ =>
+--     simp only [matchStep, IterationT.Plausible.copy, CodensityT.mapH_eq_bindH, CodensityT.bindH_assoc,
+--       IterationT.computation_pure, CodensityT.bindH_pure]
+--     rfl
