Iterator/Lemmas/Producer.lean
@@ -1,0 +1,35 @@
+import Iterator.Producers
+import Iterator.Consumers
+import Iterator.Lemmas.Consumer
+
+section ListIterator
+
+variable {m : Type v → Type v} [Monad m] {β : Type v}
+
+theorem List.step_iter_nil :
+    (([] : List β).iter m).step = pure ⟨.done, .done, rfl, rfl⟩ := by
+  simp only [iter, Iter.step, CodensityT.run, Iter.stepH, CodensityT.mapH, Iterator.step, pure,
+    Function.comp_apply, Iter.Step.ofInternal, IterationT.Plausible.map, IterStep.map, id_eq]
+  congr
+
+theorem List.step_iter_cons {x : β} {xs : List β} :
+    ((x :: xs).iter m).step = pure ⟨.yield (xs.iter m) x, .yield (xs.iter m).inner x, rfl, rfl⟩ := by
+  simp only [iter, Iter.step, CodensityT.run, Iter.stepH, CodensityT.mapH, Iterator.step, pure,
+    Function.comp_apply, Iter.Step.ofInternal, IterationT.Plausible.map, IterStep.map, id_eq]
+  congr
+
+private theorem List.toArray_iter.aux {l : List β} {acc : Array β} [LawfulMonad m] :
+    Iter.toArray.go (l.iter m) acc = pure (acc ++ l.toArray) := by
+  induction l generalizing acc with
+  | nil =>
+    rw [Iter.toArray.go]
+    simp [List.step_iter_nil]
+  | cons x xs ih =>
+    rw [Iter.toArray.go]
+    simp [List.step_iter_cons, ih]
+
+theorem List.toArray_iter {l : List β} [LawfulMonad m] :
+    Iter.toArray (l.iter m) = pure l.toArray := by
+  simp [Iter.toArray, List.toArray_iter.aux]
+
+end ListIterator
